Low-level Merkle tree: refactored some code; still working on correctness of insertion

examples/low-level/merkletree/MerkleTree.Low.fst
@@ -29,7 +29,23 @@ assume val hash_init_idem:
   h:hash -> Lemma (hash_from_hashes h hash_init = h)
 
 // This number says that the maximum number of values is (2^32 - 1)
-let max_num_elts_lg = 32
+let max_nelts_sz = 32
+
+/// Mapping sequences (why is it not in the library?)
+
+val seq_map: 
+  #a:Type -> #b:Type -> f:(a -> b) -> s:S.seq a -> 
+  Tot (fs:S.seq b{S.length fs = S.length s}) (decreases (S.length s))
+let rec seq_map #a #b f s =
+  if S.length s = 0 then S.empty
+  else S.cons (f (S.head s)) (seq_map f (S.tail s))
+
+// val seq_map_create:
+//   #a:Type -> #b:Type -> f: (a -> b) -> 
+//   len:nat -> ia:a ->
+//   Lemma (seq_map f (S.create len ia) == S.create len (f ia))
+// let rec seq_map_create #a #b f len ia =
+//   admit ()
 
 /// Allocation by power of two
 
@@ -112,16 +128,73 @@ let alloc_sz_lg_not_pow2_inc nelts =
 /// Low-level Merkle tree data structure
 
 noeq type merkle_tree =
-| MT: nelts:nat{nelts > 0 && nelts < pow2 max_num_elts_lg} -> 
+| MT: nelts:nat{nelts > 0 && nelts < pow2 max_nelts_sz} -> 
       // The value buffer will be resized when elements are added.
       // Resizing mechanism will be similar to that of C++ vector.
       values:elem_buf{B.length values = alloc_sz nelts} ->
       // The actual number of internal roots should be equal to 
       // the number of "set" bits of `nelts`.
-      iroots:hash_buf{B.length iroots = max_num_elts_lg} ->
+      iroots:hash_buf{B.length iroots = max_nelts_sz} ->
       merkle_tree
 
 let mtree_ptr = B.pointer merkle_tree
+
+/// Invariants between internal roots and values
+
+val merkle_root_of_pow2:
+  #nelts:nat{is_pow2 nelts} -> vs:hash_seq{S.length vs = nelts} -> 
+  GTot hash
+let rec merkle_root_of_pow2 #nelts vs =
+  if nelts = 1 then S.index vs 0
+  else 
+    let lrt = merkle_root_of_pow2 #(nelts / 2) (S.slice vs 0 (nelts / 2)) in
+    let rrt = merkle_root_of_pow2 #(nelts / 2) (S.slice vs (nelts / 2) nelts) in
+    hash_from_hashes lrt rrt
+
+val pow2_floor: 
+  n:nat{n > 0} -> GTot (p:nat{pow2 p <= n && n < pow2 (p + 1)})
+let rec pow2_floor n =
+  if n = 1 then 0 else 1 + pow2_floor (n / 2)
+
+val num_iroots_of: 
+  nelts_sz:nat -> nelts:nat{nelts < pow2 nelts_sz} -> 
+  GTot (nirs:nat{nirs <= nelts_sz})
+let rec num_iroots_of nelts_max_lg nelts =
+  if nelts = 0 then 0
+  else 1 + num_iroots_of (nelts_max_lg - 1) (nelts - pow2 (pow2_floor nelts))
+
+val iroots_of_hashes:
+  nelts_sz:nat -> nelts:nat{nelts < pow2 nelts_sz} -> 
+  hs:hash_seq{S.length hs = nelts} ->
+  GTot (iroots:hash_seq{S.length iroots = num_iroots_of nelts_sz nelts})
+let rec iroots_of_hashes nelts_sz nelts hs =
+  if nelts = 0 then hs
+  else S.cons (merkle_root_of_pow2 #(pow2 (pow2_floor nelts))
+				   (S.slice hs 0 (pow2 (pow2_floor nelts))))
+	      (iroots_of_hashes (nelts_sz - 1) (nelts - (pow2 (pow2_floor nelts)))
+				(S.slice hs (pow2 (pow2_floor nelts)) nelts))
+
+unfold val iroots_of: 
+  nelts_sz:nat -> nelts:nat{nelts < pow2 nelts_sz} -> 
+  es:elem_seq{S.length es = nelts} -> GTot hash_seq
+unfold let iroots_of nelts_sz nelts vs =
+  iroots_of_hashes nelts_sz nelts (seq_map hash_from_elem vs)
+
+unfold val merkle_tree_elems_wf:
+  nelts:nat{nelts > 0 && nelts < pow2 max_nelts_sz} -> 
+  values:elem_seq{S.length values = nelts} ->
+  iroots:hash_seq{S.length iroots = num_iroots_of max_nelts_sz nelts} ->
+  GTot bool
+unfold let merkle_tree_elems_wf nelts values iroots =
+  iroots_of max_nelts_sz nelts values = iroots
+
+unfold val merkle_tree_wf: HS.mem -> merkle_tree -> GTot Type0
+unfold let merkle_tree_wf h mt =
+  B.live h (MT?.values mt) /\ B.live h (MT?.iroots mt) /\
+  merkle_tree_elems_wf 
+    (MT?.nelts mt) 
+    (S.slice (B.as_seq h (MT?.values mt)) 0 (MT?.nelts mt))
+    (S.slice (B.as_seq h (MT?.iroots mt)) 0 (num_iroots_of max_nelts_sz (MT?.nelts mt)))
 
 /// Initialization
 
@@ -129,11 +202,16 @@ val create_merkle_tree: unit ->
   HST.ST merkle_tree
 	 (requires (fun _ -> true))
 	 (ensures (fun h0 mt h1 -> 
-	   B.live h1 (MT?.values mt) /\ B.freeable (MT?.values mt) /\
-	   B.live h1 (MT?.iroots mt)))
+	   B.freeable (MT?.values mt) /\ 
+	   B.disjoint (MT?.values mt) (MT?.iroots mt) /\
+	   merkle_tree_wf h1 mt))
 let create_merkle_tree _ =
-  MT 1 (B.malloc root elem_init 1ul)
-     (B.malloc root hash_init (UInt32.uint_to_t max_num_elts_lg))
+  let values = B.malloc root elem_init 1ul in
+  let iroots = B.malloc root (hash_from_elem elem_init) (UInt32.uint_to_t max_nelts_sz) in
+  // let hh = HST.get () in
+  // assume (B.disjoint values iroots);
+  // assume (iroots_of max_nelts_sz 1 (S.slice (B.as_seq hh values) 0 1) = S.slice (B.as_seq hh iroots) 0 1);
+  admit (); MT 1 values iroots
 
 // val init_merkle_tree: unit -> HST.St mtree_ptr
 // let init_merkle_tree _ =
@@ -142,11 +220,11 @@ let create_merkle_tree _ =
 /// Insertion
 
 val mt_is_full: merkle_tree -> Tot bool
-let mt_is_full mt = MT?.nelts mt >= pow2 max_num_elts_lg - 1
+let mt_is_full mt = MT?.nelts mt >= pow2 max_nelts_sz - 1
 
 unfold val insert_nelts: 
-  nelts:nat{nelts < pow2 max_num_elts_lg - 1} ->
-  Tot (inelts:nat{inelts < pow2 max_num_elts_lg})
+  nelts:nat{nelts < pow2 max_nelts_sz - 1} ->
+  Tot (inelts:nat{inelts < pow2 max_nelts_sz})
 unfold let insert_nelts nelts =
   nelts + 1
 
@@ -159,7 +237,7 @@ let rec pow2_lt_le n p =
   else pow2_lt_le (n / 2) (p - 1)
 
 val insert_values:
-  nelts:nat{nelts > 0 && nelts < pow2 max_num_elts_lg - 1} -> 
+  nelts:nat{nelts > 0 && nelts < pow2 max_nelts_sz - 1} -> 
   vs:elem_buf{B.length vs = alloc_sz nelts} ->
   e:elem -> 
   HST.ST (ivs:elem_buf{B.length ivs = alloc_sz (insert_nelts nelts)})
@@ -173,7 +251,7 @@ let insert_values nelts vs e =
   if is_pow2 (nelts + 1)
   then (let hh0 = HST.get () in
        // Need to prove `2 * nelts + 1` does not exceed the maximum before `B.malloc`
-       pow2_lt_le (nelts + 1) max_num_elts_lg; 
+       pow2_lt_le (nelts + 1) max_nelts_sz; 
        let nvs = B.malloc root elem_init (UInt32.uint_to_t (2 * nelts + 1)) in
 
        // `blit` requires two buffers to be disjoint
@@ -194,15 +272,49 @@ let insert_values nelts vs e =
        alloc_sz_lg_not_pow2_inc nelts;
        vs)
 
-val merkle_root_of_pow2:
-  #nelts:nat{is_pow2 nelts} -> vs:hash_seq{S.length vs = nelts} -> 
-  GTot hash
-let rec merkle_root_of_pow2 #nelts vs =
-  if nelts = 1 then S.index vs 0
-  else 
-    let lrt = merkle_root_of_pow2 #(nelts / 2) (S.slice vs 0 (nelts / 2)) in
-    let rrt = merkle_root_of_pow2 #(nelts / 2) (S.slice vs (nelts / 2) nelts) in
-    hash_from_hashes lrt rrt
+// TODO: How to declare `values` as a ghost variable?
+#set-options "--z3rlimit 20"
+val insert_iroots:
+  nelts:nat{nelts > 0 && nelts < pow2 max_nelts_sz - 1} ->
+  values:elem_buf{B.length values = alloc_sz nelts} ->
+  irs:hash_buf{B.length irs = max_nelts_sz} ->
+  nv:elem ->
+  HST.ST unit
+	 (requires (fun h0 ->
+	   B.live h0 values /\ B.live h0 irs /\ B.disjoint values irs /\
+	   merkle_tree_elems_wf 
+	     nelts (S.slice (B.as_seq h0 values) 0 nelts)
+	     (S.slice (B.as_seq h0 irs) 0 (num_iroots_of max_nelts_sz nelts))))
+	 (ensures (fun h0 _ h1 ->
+	   modifies (loc_buffer irs) h0 h1 /\
+	   merkle_tree_elems_wf
+	     (insert_nelts nelts)
+	     (S.append (S.slice (B.as_seq h0 values) 0 nelts) (S.create 1 nv))
+	     (S.slice (B.as_seq h1 irs) 0 (num_iroots_of max_nelts_sz (insert_nelts nelts)))))
+let rec insert_iroots nelts values irs nv =
+  admit ()
+
+val insert: 
+  mt:merkle_tree -> e:elem -> 
+  HST.ST merkle_tree
+	 (requires (fun h0 -> 
+	   MT?.nelts mt < pow2 max_nelts_sz - 1 /\
+	   B.disjoint (MT?.values mt) (MT?.iroots mt) /\
+	   B.live h0 (MT?.values mt) /\ B.freeable (MT?.values mt) /\
+	   B.live h0 (MT?.iroots mt) /\ B.freeable (MT?.iroots mt) /\
+	   ~ (mt_is_full mt) /\
+	   merkle_tree_wf h0 mt))
+	 (ensures (fun h0 nmt h1 -> true))
+let insert mt e =
+  let nnelts = insert_nelts (MT?.nelts mt) in
+  let niroots = (insert_iroots (MT?.nelts mt) (MT?.values mt) (MT?.iroots mt) e; MT?.iroots mt) in
+  let nvalues = insert_values (MT?.nelts mt) (MT?.values mt) e in
+  assert (nnelts > 0 && nnelts < pow2 max_nelts_sz);
+  assert (B.length nvalues = alloc_sz nnelts);
+  assert (B.length niroots = max_nelts_sz);
+  admit () // MT nnelts nvalues niroots
+
+/// Getting the Merkle root
 
 val padding_to_pow2:
   nelts:nat{nelts > 0} -> GTot (sz:nat{
@@ -228,101 +340,53 @@ let merkle_root_of_hashes vs =
   merkle_root_of_pow2 #(pow2 (padding_to_pow2 (S.length vs))) 
 		      (pad_hashes_pow2 vs)
 
-val pow2_floor: 
-  n:nat{n > 0} -> GTot (p:nat{pow2 p <= n && n < pow2 (p + 1)})
-let rec pow2_floor n =
-  if n = 1 then 0 else 1 + pow2_floor (n / 2)
+val merkle_root_of_iroots_seq':
+  acc:hash ->
+  nirs:nat{nirs <= max_nelts_sz} ->
+  irs:hash_seq{S.length irs = max_nelts_sz} -> 
+  GTot hash (decreases nirs)
+let rec merkle_root_of_iroots_seq' acc nirs irs =
+  if nirs = 0 then acc
+  else merkle_root_of_iroots_seq'
+       (hash_from_hashes (S.index irs (nirs - 1)) acc)
+       (nirs - 1) irs
 
-val num_iroots_of: nelts:nat -> GTot nat
-let rec num_iroots_of nelts =
-  if nelts = 0 then 0
-  else 1 + num_iroots_of (nelts - pow2 (pow2_floor nelts))
+val merkle_root_of_iroots':
+  acc:hash ->
+  nirs:nat{nirs <= max_nelts_sz} ->
+  irs:hash_buf{B.length irs = max_nelts_sz} -> 
+  HST.ST hash
+	 (requires (fun h0 -> B.live h0 irs))
+	 (ensures (fun h0 hs h1 -> 
+	   h1 == h0 /\
+	   merkle_root_of_iroots_seq' acc nirs (B.as_seq h0 irs) = hs))
+let rec merkle_root_of_iroots' acc nirs irs =
+  if nirs = 0 then acc
+  else merkle_root_of_iroots'
+       (hash_from_hashes (B.index irs (UInt32.uint_to_t (nirs - 1))) acc)
+       (nirs - 1) irs
 
-val num_iroots_of_limit:
-  nelts_max_lg:nat -> nelts:nat{nelts < pow2 nelts_max_lg} ->
-  Lemma (num_iroots_of nelts <= nelts_max_lg)
-let rec num_iroots_of_limit nelts_max_lg nelts =
-  if nelts = 0 then ()
-  else num_iroots_of_limit 
-       (nelts_max_lg - 1) 
-       (nelts - pow2 (pow2_floor nelts))
+val merkle_root_of_iroots_seq:
+  nirs:nat{nirs <= max_nelts_sz} ->
+  irs:hash_seq{S.length irs = max_nelts_sz} -> 
+  GTot hash (decreases nirs)
+let rec merkle_root_of_iroots_seq nirs irs =
+  merkle_root_of_iroots_seq' hash_init nirs irs
 
-// val num_iroots_of_inv:
-//   nelts:nat{nelts > 0} ->
-//   Lemma (num_iroots_of nelts = 
+val merkle_root_of_iroots:
+  nirs:nat{nirs <= max_nelts_sz} ->
+  irs:hash_buf{B.length irs = max_nelts_sz} -> 
+  HST.ST hash
+	 (requires (fun h0 -> B.live h0 irs))
+	 (ensures (fun h0 hs h1 -> 
+	   h1 == h0 /\
+	   merkle_root_of_iroots_seq nirs (B.as_seq h0 irs) = hs))
+let merkle_root_of_iroots nirs irs =
+  merkle_root_of_iroots' hash_init nirs irs
 
-// val merkle_root_of_iroots: 
-//   nelts:nat{nelts > 0} -> 
-//   iroots:hash_seq{S.length iroots = num_iroots_of nelts} ->
-//   GTot hash
-// let rec merkle_root_of_iroots nelts iroots =
-//   if nelts = 1 then S.index iroots 0
-//   else if nelts % 2 = 0 then 
-
-val iroots_of_hashes:
-  nelts:nat -> hs:hash_seq{S.length hs = nelts} ->
-  GTot (iroots:hash_seq{S.length iroots = num_iroots_of nelts})
-let rec iroots_of_hashes nelts hs =
-  if nelts = 0 then hs
-  else S.cons (merkle_root_of_pow2 #(pow2 (pow2_floor nelts))
-				   (S.slice hs 0 (pow2 (pow2_floor nelts))))
-	      (iroots_of_hashes (nelts - (pow2 (pow2_floor nelts)))
-			 (S.slice hs (pow2 (pow2_floor nelts)) nelts))
-
-val seq_map: 
-  #a:Type -> #b:Type -> (f: a -> b) -> s:S.seq a -> 
-  Tot (fs:S.seq b{S.length fs = S.length s}) (decreases (S.length s))
-let rec seq_map #a #b f s =
-  if S.length s = 0 then S.empty
-  else S.cons (f (S.head s)) (seq_map f (S.tail s))
-
-unfold val iroots_of: 
-  nelts:nat -> es:elem_seq{S.length es = nelts} -> GTot hash_seq
-unfold let iroots_of nelts vs =
-  iroots_of_hashes nelts (seq_map hash_from_elem vs)
-
-// How to declare `values` as a ghost variable?
-#set-options "--z3rlimit 20"
-val insert_iroots:
-  nelts:nat{nelts > 0 && nelts < pow2 max_num_elts_lg - 1} ->
-  values:elem_buf{B.length values = alloc_sz nelts} ->
-  irs:hash_buf{B.length irs = max_num_elts_lg} ->
-  nv:elem ->
-  HST.ST unit
-	 (requires (fun h0 ->
-	   B.live h0 values /\ B.live h0 irs /\ B.disjoint values irs /\
-	   (num_iroots_of_limit max_num_elts_lg nelts;
-	     iroots_of nelts (S.slice (B.as_seq h0 values) 0 nelts) =
-	     S.slice (B.as_seq h0 irs) 0 (num_iroots_of nelts))))
-	 (ensures (fun h0 _ h1 ->
-	   modifies (loc_buffer irs) h0 h1 /\
-	   (num_iroots_of_limit max_num_elts_lg (nelts + 1);
-	     iroots_of (nelts + 1) (S.append (S.slice (B.as_seq h0 values) 0 nelts) (S.create 1 nv)) =
-	     S.slice (B.as_seq h1 irs) 0 (num_iroots_of (nelts + 1)))))
-let rec insert_iroots nelts values irs nv =
-  admit ()
-
-val insert: 
-  mt:merkle_tree -> e:elem -> 
-  HST.ST merkle_tree
-	 (requires (fun h0 -> 
-	   MT?.nelts mt < pow2 max_num_elts_lg - 1 /\
-	   B.disjoint (MT?.values mt) (MT?.iroots mt) /\
-	   B.live h0 (MT?.values mt) /\ B.freeable (MT?.values mt) /\
-	   B.live h0 (MT?.iroots mt) /\ B.freeable (MT?.iroots mt) /\
-	   ~ (mt_is_full mt) /\
-	   (num_iroots_of_limit max_num_elts_lg (MT?.nelts mt);
-	     iroots_of (MT?.nelts mt) (S.slice (B.as_seq h0 (MT?.values mt)) 0 (MT?.nelts mt)) =
-	     S.slice (B.as_seq h0 (MT?.iroots mt)) 0 (num_iroots_of (MT?.nelts mt)))))
-	 (ensures (fun h0 _ h1 -> true))
-let insert mt e =
-  let nnelts = insert_nelts (MT?.nelts mt) in
-  let niroots = (insert_iroots (MT?.nelts mt) (MT?.values mt) (MT?.iroots mt) e; MT?.iroots mt) in
-  let nvalues = insert_values (MT?.nelts mt) (MT?.values mt) e in
-  assert (nnelts > 0 && nnelts < pow2 max_num_elts_lg);
-  assert (B.length nvalues = alloc_sz nnelts);
-  assert (B.length niroots = max_num_elts_lg);
-  admit () // MT nnelts nvalues niroots
-
-/// Getting the Merkle root
+val merkle_root_of_iroots_ok:
+  h:HS.mem -> mt:merkle_tree ->
+  Lemma (requires (merkle_tree_wf h mt))
+	(ensures (merkle_root_of_iroots_seq (num_iroots_of max_nelts_sz (MT?.nelts mt)) (B.as_seq h (MT?.iroots mt)) =
+		 merkle_root_of_hashes (seq_map hash_from_elem (B.as_seq h (MT?.values mt)))))
 
